make sure "demo" also works on 32bit, not just 12bit

src/PipelineDemoStepwise.v
@@ -16,30 +16,32 @@ Require Import compiler.Machine.
 Require Import compiler.StateMonad.
 Require Import compiler.runsToSatisfying.
 Require Import compiler.MyOmega.
+Require Import compiler.zcast.
 
 Definition myvar := nat.
 Definition var_x1: myvar := 3.
 Definition var_x2: myvar := 4.
 Definition var_i: myvar := 5.
-Definition w := 12. (* bit width *)
 Definition wlit := 12. (* bit width of literals *)
 Definition wjimm := 12. (* bit width of jump-immediates *)
-Definition wdiff := 0. (* difference between literals width and full width *)
-
-(*
-Too big for evaluation inside Coq:
-Definition w := 32. (* bit width *)
-Definition wlit := 12. (* bit width of literals *)
 Definition wdiff := 20. (* difference between literals width and full width *)
-*)
+Notation w := (wlit + wdiff). (* bit width *)
+
+Lemma my_bound: wlit + wdiff >= wjimm. cbv. omega. Qed.
+
+(* Otherwise "Eval cbv" and "reflexivity" take forever *)
+Opaque wlit wjimm wdiff.
 
 Definition empty_types: member (@nil myvar) -> type. intro. inversion H. Defined.
 Definition empty_vals: forall m : member (@nil myvar), @interp_type w (empty_types m).
   intro. inversion m. Defined.
 
-Definition p1_LLG(n: word w): word w :=
+Definition signed_lit_to_word(v: word wlit): word w := nat_cast word eq_refl (sext v wdiff).
+
+Definition p1_LLG(n: word wlit): word w :=
+  let n' := signed_lit_to_word n in
   let x1 := $0 in
-  for i from 0 to n updating (x1) {{
+  for i from 0 to n' updating (x1) {{
      let x2 := x1 ^+ i ^* i in
      x2
   }} ;;
@@ -52,9 +54,10 @@ Definition i_in_ix1: member [var_i; var_x1]. apply member_here. Defined.
 Definition x1_in_x1: member [var_x1]. apply member_here. Defined.
 Definition x2_in_x2ix1: member [var_x2; var_i; var_x1]. apply member_here. Defined.
 
-Definition p1_LLG_ast(n: word w): expr (@nil myvar) empty_types TInt :=
+Definition p1_LLG_ast(n: word wlit): @expr w myvar [] empty_types TInt :=
+  let n' := signed_lit_to_word n in
   ELet var_x1 (ELit $0)
-  (EFor var_i (ELit n) x1_in_x1
+  (EFor var_i (ELit n') x1_in_x1
      (ELet var_x2 (EOp (EVar x1_in_ix1) OPlus (EOp (EVar i_in_ix1) OTimes (EVar i_in_ix1)))
      (EVar x2_in_x2ix1))
   (EVar x1_in_x1)).
@@ -62,27 +65,42 @@ Definition p1_LLG_ast(n: word w): expr (@nil myvar) empty_types TInt :=
 Definition interp_expr'{t}(e: expr (@nil myvar) empty_types t): interp_type t :=
   interp_expr e empty_vals.
 
-Goal forall n, p1_LLG n = interp_expr' (p1_LLG_ast n). intros. reflexivity. Qed.
-
-Goal forall n, p1_LLG n = interp_expr' (p1_LLG_ast n).
-  intros. unfold p1_LLG. unfold interp_expr', interp_expr. cbn. reflexivity.
-Qed.
+Goal forall (n: word wlit), p1_LLG n = interp_expr' (p1_LLG_ast n).
+Proof. intros. reflexivity. Qed.
 
 Definition nameGenState_initial: myvar := 10. (* should be bigger than all vars used in source *)
 
+(* TODO this is a stmt where each literal is cast from wlit to w, so the its literal width is
+   already w instead of wlit *)
 Definition compileLLG2FlatImp{l G t}(e: expr l G t): @stmt w myvar * myvar :=
   fst (LLG2FlatImp.compile nameGenState_initial e).
 
 Definition p1_FlatImp(n: word wlit): @stmt w myvar * myvar := compileLLG2FlatImp (p1_LLG_ast n).
 
-Definition p1_FlatImp'(n: word wlit): @stmt w myvar * myvar :=
-  ltac:(let r := eval cbv -[natToWord] in (p1_FlatImp n) in exact r).
+Definition p1_FlatImp'(n: word wlit): @stmt wlit myvar * myvar.
+  set (r := compileLLG2FlatImp (p1_LLG_ast n)).
+  cbv -[natToWord signed_lit_to_word Nat.add] in r.
+  (* copy-pasting and removing signed_lit_to_word changes implicit argument for literal bit width *)
+  exact (SSeq (SLit 10 $ (0))
+        (SSeq (SSet 3 10)
+           (SSeq (SLit 20 $ (1))
+              (SSeq (SLit 11 n)
+                 (SSeq (SLit 5 $ (0))
+                    (SSeq
+                       (SLoop (SOp 12 OLt 5 11) 12
+                          (SSeq
+                             (SSeq
+                                (SSeq (SSet 13 3)
+                                   (SSeq (SSeq (SSet 14 5) (SSeq (SSet 15 5) (SOp 16 OTimes 14 15)))
+                                      (SOp 17 OPlus 13 16))) (SSeq (SSet 4 17) (SSet 18 4)))
+                             (SSeq (SSet 3 18) (SOp 5 OPlus 5 20)))) (SSet 19 3)))))), 19).
+Defined.
 
-Definition p1_FlatImp_stmt(n: word wlit): @stmt w myvar := 
-  ltac:(let r := eval cbv -[natToWord] in (fst (p1_FlatImp n)) in exact r).
+Definition p1_FlatImp_stmt(n: word wlit): @stmt wlit myvar := 
+  ltac:(let r := eval cbv [fst p1_FlatImp'] in (fst (p1_FlatImp' n)) in exact r).
 
 Definition p1_FlatImp_resVar(n: word wlit): myvar := 
-  ltac:(let r := eval cbv -[natToWord] in (snd (p1_FlatImp n)) in exact r).
+  ltac:(let r := eval cbv [snd p1_FlatImp'] in (snd (p1_FlatImp' n)) in exact r).
 
 Definition lotsOfFuel := 100.
 
@@ -98,12 +116,12 @@ Definition eval_FlatImp_stmt(s: @stmt wlit myvar * myvar): option (word w) :=
 
 Transparent wlt_dec.
 
-Goal eval_FlatImp_stmt (p1_FlatImp $4) = Some $14. reflexivity. Qed.
+Goal eval_FlatImp_stmt (p1_FlatImp' $4) = Some $14. reflexivity. Qed.
 
-Definition compileFlat2Riscv(f: @stmt w myvar): list (@Instruction wlit wjimm myvar) :=
+Definition compileFlat2Riscv(f: @stmt wlit myvar): list (@Instruction wlit wjimm myvar) :=
   compiler.FlatToRiscv.compile_stmt f.
 
-Definition p1_riscv(n: word w): list (@Instruction wlit wjimm myvar) :=
+Definition p1_riscv(n: word wlit): list (@Instruction wlit wjimm myvar) :=
   compileFlat2Riscv (p1_FlatImp_stmt n).
 
 Goal False. set (r := p1_riscv $3). cbv in *. Abort.
@@ -112,8 +130,6 @@ Definition lotsOfFuel_lowlevel := 100.
 
 Definition myInst := (@IsRiscvMachine wlit wdiff wjimm myvar _).
 Existing Instance myInst.
-
-Lemma my_bound: wlit + wdiff >= wjimm. cbv. omega. Qed.
 
 Definition runThenGet(resVar: myvar):
   State (@RiscvMachine wlit wdiff wjimm myvar) (word (wlit+wdiff)) :=
@@ -132,12 +148,7 @@ Proof.
   intros. inversion H.
 Qed.
 
-(*
-Axiom flat_src_correct: forall n, exists fuelH finalH,
-  eval_stmt fuelH empty_state (p1_FlatImp_stmt $ (n)) = Success finalH.
-*)
-
-
+Transparent wlit wjimm wdiff.
 
 Lemma p1_runs_correctly_1: forall n resVar fuelH finalH,
   eval_stmt (wdiff:=wdiff) (wlit:=wlit) (w_eq:=eq_refl) fuelH empty_state (p1_FlatImp_stmt $ (n)) = Success finalH ->
